src/ListMemory.v
@@ -46,22 +46,7 @@ Section Memory.
 
   Definition zero_mem: nat -> mem := const_mem $0.
 
-  Definition valid_addr(m: mem)(alignment: nat)(addr: word w): Prop :=
-    wordToNat addr + alignment <= mem_size m /\
-    (wordToNat addr) mod alignment = 0.
-
 End Memory.
-
-Instance mem_is_Memory(w: nat): Memory mem (word w) := {|
-  loadByte    := read_byte;
-  loadHalf    := read_half;
-  loadWord    := read_word;
-  loadDouble  := read_double;
-  storeByte   := write_byte;
-  storeHalf   := write_half;
-  storeWord   := write_word;
-  storeDouble := write_double;
-|}.
 
 Local Ltac wrap L :=
   intros;
@@ -74,74 +59,27 @@ Local Ltac wrap L :=
   try apply wordToNat_neq1;
   (congruence || omega || idtac).    
 
-Lemma write_read_byte_eq: forall w m (a1 a2: word w) v,
-    valid_addr m 1 a1 ->
-    a2 = a1 ->
-    read_byte (write_byte m a1 v) a2 = v.
-Proof. wrap ListMemoryNatAddr.write_read_byte_eq. Qed.
-
-Lemma write_read_byte_ne: forall w m (a1 a2: word w) v,
-    valid_addr m 1 a1 ->
-    valid_addr m 1 a2 ->
-    a2 <> a1 ->
-    read_byte (write_byte m a1 v) a2 = read_byte m a2.
-Proof. wrap ListMemoryNatAddr.write_read_byte_ne. Qed.
-
-Lemma write_byte_preserves_mem_size: forall w m (a: word w) v,
-    valid_addr m 1 a ->
-    mem_size (write_byte m a v) = mem_size m.
-Proof. wrap ListMemoryNatAddr.write_byte_preserves_mem_size. Qed.
-
-Lemma write_read_half_eq: forall w m (a1 a2: word w) v,
-    valid_addr m 2 a1 ->
-    a2 = a1 ->
-    read_half (write_half m a1 v) a2 = v.
-Proof. wrap ListMemoryNatAddr.write_read_half_eq. Qed.
-
-Lemma write_read_half_ne: forall w m (a1 a2: word w) v,
-    valid_addr m 2 a1 ->
-    valid_addr m 2 a2 ->
-    a2 <> a1 ->
-    read_half (write_half m a1 v) a2 = read_half m a2.
-Proof. wrap ListMemoryNatAddr.write_read_half_ne. Qed.
-
-Lemma write_half_preserves_mem_size: forall w m (a: word w) v,
-    valid_addr m 2 a ->
-    mem_size (write_half m a v) = mem_size m.
-Proof. wrap ListMemoryNatAddr.write_half_preserves_mem_size. Qed.
-
-Lemma write_read_word_eq: forall w m (a1 a2: word w) v,
-    valid_addr m 4 a1 ->
-    a2 = a1 ->
-    read_word (write_word m a1 v) a2 = v.
-Proof. wrap ListMemoryNatAddr.write_read_word_eq. Qed.
-
-Lemma write_read_word_ne: forall w m (a1 a2: word w) v,
-    valid_addr m 4 a1 ->
-    valid_addr m 4 a2 ->
-    a2 <> a1 ->
-    read_word (write_word m a1 v) a2 = read_word m a2.
-Proof. wrap ListMemoryNatAddr.write_read_word_ne. Qed.
-
-Lemma write_word_preserves_mem_size: forall w m (a: word w) v,
-    valid_addr m 4 a ->
-    mem_size (write_word m a v) = mem_size m.
-Proof. wrap ListMemoryNatAddr.write_word_preserves_mem_size. Qed.
-
-Lemma write_read_double_eq: forall w m (a1 a2: word w) v,
-    valid_addr m 8 a1 ->
-    a2 = a1 ->
-    read_double (write_double m a1 v) a2 = v.
-Proof. wrap ListMemoryNatAddr.write_read_double_eq. Qed.
-
-Lemma write_read_double_ne: forall w m (a1 a2: word w) v,
-    valid_addr m 8 a1 ->
-    valid_addr m 8 a2 ->
-    a2 <> a1 ->
-    read_double (write_double m a1 v) a2 = read_double m a2.
-Proof. wrap ListMemoryNatAddr.write_read_double_ne. Qed.
-
-Lemma write_double_preserves_mem_size: forall w m (a: word w) v,
-    valid_addr m 8 a ->
-    mem_size (write_double m a v) = mem_size m.
-Proof. wrap ListMemoryNatAddr.write_double_preserves_mem_size. Qed.
+Instance mem_is_Memory(w: nat): Memory mem w := {|
+  memSize     := mem_size;
+  loadByte    := read_byte;
+  loadHalf    := read_half;
+  loadWord    := read_word;
+  loadDouble  := read_double;
+  storeByte   := write_byte;
+  storeHalf   := write_half;
+  storeWord   := write_word;
+  storeDouble := write_double;
+|}.
+- wrap ListMemoryNatAddr.write_read_byte_eq.
+- wrap ListMemoryNatAddr.write_read_byte_ne.
+- wrap ListMemoryNatAddr.write_byte_preserves_mem_size.
+- wrap ListMemoryNatAddr.write_read_half_eq.
+- wrap ListMemoryNatAddr.write_read_half_ne.
+- wrap ListMemoryNatAddr.write_half_preserves_mem_size.
+- wrap ListMemoryNatAddr.write_read_word_eq.
+- wrap ListMemoryNatAddr.write_read_word_ne.
+- wrap ListMemoryNatAddr.write_word_preserves_mem_size.
+- wrap ListMemoryNatAddr.write_read_double_eq.
+- wrap ListMemoryNatAddr.write_read_double_ne.
+- wrap ListMemoryNatAddr.write_double_preserves_mem_size.
+Defined.
